proof/SomeDKC.ec
@@ -50,7 +50,7 @@ theory SomeDKC.
   lemma w2kw_kw2w w b : fst (w2kw (kw2w w b)) = w. 
   proof.
     simplify w2kw kw2w fst.
-    case b => hc.
+    case b => hc. 
     smt tmo=60.
     simplify.
     smt tmo=60.
@@ -98,12 +98,6 @@ theory SomeDKC.
     smt tmo=60.
   qed.
   
-  (*op w2kw'(w) =
-  (*if w = witness then witness else*)
-  let kwi = (W.to_int w) %/ 2 (* / 2 *)
-                          in let lsbi = W.getlsb w
-                          in KW.from_int kwi.*)
-  
   clone import SomePRF.PRF with
 	type D = word,
 	type R = word,
@@ -119,9 +113,7 @@ theory SomeDKC.
         type cipher_t = word,
         op E(t,k1,k2,m) = (F (fst (w2kw k1)) t) ^ (F (fst (w2kw k2)) t) ^ m,
         op D(t,k1,k2,c) = (F (fst (w2kw k1)) t) ^ (F (fst (w2kw k2)) t) ^ c.
-        
-  (*prover ["Z3"].*)
-        
+                
   (** DKC security definitions, instantiated with the words defined in W *)
   clone import DKCSec2.DKCSecurity with
     (*theory WD <- W,*)
@@ -130,7 +122,7 @@ theory SomeDKC.
 
   lemma PrfDKC_correct : PrfDKC.Correct().
   proof.
-    simplify Correct E D => t k1 k2 x;smt.
+    by simplify Correct E D => t k1 k2 x; smt.
   qed.
   
   (*  Prove that for all l, there exists a PRF attacker that breaks
@@ -139,9 +131,7 @@ theory SomeDKC.
       the PRF oracle. If its the real oracle, then we are in the DKC
       game; otherwise, we are in a OTP world, because tweaks do not
       repeat. *)
-   
-  (*op bound: int.*)
-  
+     
   (*************************************)
   (** DKC PART *)
   (*************************************)
@@ -166,6 +156,7 @@ theory SomeDKC.
       DKCp.b = b;
       DKCp.l = l;
       DKCp.lsb = witness;
+      DKCp.ksec = witness;
       DKCp.used = FSet.fset0;
       DKCp.kpub = map0;
       
@@ -206,7 +197,7 @@ theory SomeDKC.
       ans = bad;
       (rn,ib,jb,lb,t) = q;
       
-      if (!(mem DKCp.used t) && 0 <= ib.`1 /\ ib.`1 < jb.`1 && jb.`1 < lb.`1 && lb.`1 < bound /\ lb <> (DKCp.l,DKCp.lsb)) {
+      if (!(mem DKCp.used t) /\ 0 <= ib.`1 /\ ib.`1 < jb.`1 /\ jb.`1 < lb.`1 /\ lb.`1 < bound /\ lb <> (DKCp.l,DKCp.lsb)) {
         DKCp.used = DKCp.used `|` fset1 t; (* to do: check unicity *)
         
         ki = oget DKCp.kpub.[ib];
@@ -268,7 +259,7 @@ theory SomeDKC.
       ans = bad;
       (rn,ib,jb,lb,t) = q;
   
-      if (!(mem Param.used t) && 0 <= ib.`1 /\ ib.`1 < jb.`1 && jb.`1 < lb.`1 && lb.`1 < bound /\ lb <> (Param.l,Param.lsb)) {
+      if (!(mem Param.used t) /\ 0 <= ib.`1 /\ ib.`1 < jb.`1 /\ jb.`1 < lb.`1 /\ lb.`1 < bound /\ lb <> (Param.l,Param.lsb)) {
         Param.used = Param.used `|` fset1 t; 
         
         (ki,lsbi) = oget Param.kpub.[ib];
@@ -359,7 +350,7 @@ theory SomeDKC.
   
 equiv true_key lp (A <:  Adv_DKC_t{Param,DKCp,PRFr_Wrapped}):
     DKCSecurity.Game(DKC_O,A).game ~
-    IND(PRFr_Wrapped,D(A)).main : ={glob A} /\ 0 <= lp < bound /\ b{1} /\ l{1} = lp /\ l{2} = lp
+    IND(PRFr_Wrapped,D(A)).main : ={glob A} /\ 0 <= lp < boundl /\ b{1} /\ l{1} = lp /\ l{2} = lp
                                ==> ={res}.
     proof.
       proc.
@@ -369,22 +360,16 @@ equiv true_key lp (A <:  Adv_DKC_t{Param,DKCp,PRFr_Wrapped}):
       DKCp.l{1} = Param.l{2} /\ DKCp.l{1} = lp /\ Param.l{2} = l0{2} /\ DKCp.l{1} = l{1} /\
       DKCp.lsb{1} = Param.lsb{2} /\ DKCp.ksec{1} = kw2w PRFr_Wrapped.k{2} Param.lsb{2} /\ getlsb DKCp.ksec{1} = DKCp.lsb{1} /\ lsb{1} = DKCp.lsb{1} /\ lsb{2} = Param.lsb{2} /\
       Param.tbl{2} = map0 /\
-
-      (*oget Param.kpub{2}.[(Param.l{2},Param.lsb{2})] = (witness,witness) /\
-      oget DKCp.kpub{1}.[(DKCp.l{1},DKCp.lsb{1})] = witness /\*)
       oget DKCp.kpub{1}.[(DKCp.l{1},DKCp.lsb{1})] = kw2w (fst (oget Param.kpub{2}.[(Param.l{2},Param.lsb{2})])) Param.lsb{2} /\
       (*snd (oget Param.kpub{2}.[(Param.l{2},Param.lsb{2})]) = Param.lsb{2} /\*)
       (forall k b, 0 <= k < bound => k <> Param.l{2} => oget DKCp.kpub{1}.[(k,b)] = kw2w (fst (oget Param.kpub{2}.[(k,b)])) b) /\
       (forall k b, 0 <= k < bound => snd (oget Param.kpub{2}.[(k,b)]) = b) /\
       (forall k, 0 <= k < bound => k = Param.l{2} => oget DKCp.kpub{1}.[(k,!Param.lsb{2})] = kw2w (fst (oget Param.kpub{2}.[(k,!Param.lsb{2})])) (!Param.lsb{2}))
-
-
-
-    );   
+      ); 
       inline DKC_O.initialize D(A, PRFr_Wrapped).initialize.
 
-    splitwhile{1} 11 : i < DKCp.l. 
-    splitwhile{1} 12 : i = DKCp.l.
+    splitwhile{1} 12 : i < DKCp.l. 
+    splitwhile{1} 13 : i = DKCp.l.
 
     splitwhile{2} 12 : i < Param.l. 
     splitwhile{2} 13 : i = Param.l.
@@ -409,12 +394,19 @@ equiv true_key lp (A <:  Adv_DKC_t{Param,DKCp,PRFr_Wrapped}):
     auto; progress; first 2 by idtac=>/#. rewrite !getP => /#. 
         rewrite !getP. case ((k, b1) = (i{2}, true)) => hc. rewrite !oget_some kw2w_w2kw. rewrite (Dword.lsb_dwordLsb (true) _). done. idtac=>/#. done. case ((k, b1) = (i{2}, false)) => hc'. rewrite !oget_some kw2w_w2kw. rewrite (Dword.lsb_dwordLsb (false) _). done. idtac=>/#. done. idtac=>/#.
         rewrite !getP. case ((k, b1) = (i{2}, true)) => hc. rewrite oget_some. simplify w2kw snd. rewrite (Dword.lsb_dwordLsb (true) _). done. idtac=>/#. case ((k, b1) = (i{2}, false)) => hc'. rewrite oget_some. simplify w2kw snd. rewrite (Dword.lsb_dwordLsb (false) _). done. idtac=>/#. idtac=>/#. 
-        rewrite !getP => /#. 
+        rewrite !getP => /#. (*
+        rewrite !dom_set. rewrite !in_fsetU. case (k = i{2}) => hki. case (b1) => hb1. right. rewrite in_fset1. done. left. right. rewrite in_fset1. done. left. left. rewrite H10. idtac=>/#. done. 
+        rewrite !dom_set. rewrite !in_fsetU. case (k = i{2}) => hki. case (b1) => hb1. right. rewrite in_fset1. done. left. right. rewrite in_fset1. done. left. left. rewrite H11. idtac=>/#. done. 
+        rewrite !dom_set. rewrite !in_fsetU. left. left. rewrite H12. idtac=>/#. done.  
+        rewrite !dom_set. rewrite !in_fsetU. left. left. rewrite H13. idtac=>/#. done. 
+        move : H22. rewrite !dom_set. rewrite !in_fsetU. progress. cut ? : forall (k : int) (b : bool), mem (dom DKCp.kpub{1}) (k, b) => 0 <= k by idtac=>/#. case (b1) => hb1. elim H22. progress. elim H22. progress. rewrite (H23 k b1). done. progress. smt. progress. smt. elim H22. progress. elim H22. progress. rewrite (H23 k b1). done. progress. smt. progress. smt. 
+        move : H22. rewrite !dom_set. rewrite !in_fsetU. progress. cut ? : forall (k : int) (b : bool), mem (dom DKCp.kpub{1}) (k, b) => k < bound by idtac=>/#. case (b1) => hb1. elim H22. progress. elim H22. progress. rewrite (H24 k b1). done. progress. smt. progress. smt. elim H22. progress. elim H22. progress. rewrite (H24 k b1). done. progress. smt. progress. smt. 
+        move : H22. rewrite !dom_set. rewrite !in_fsetU. progress. cut ? : forall (k : int) (b : bool), mem (dom Param.kpub{2}) (k, b) => 0 <= k by idtac=>/#. case (b1) => hb1. elim H22. progress. elim H22. progress. rewrite (H23 k b1). done. progress. smt. progress. smt. elim H22. progress. elim H22. progress. rewrite (H23 k b1). done. progress. smt. progress. smt. 
+        move : H22. rewrite !dom_set. rewrite !in_fsetU. progress. cut ? : forall (k : int) (b : bool), mem (dom Param.kpub{2}) (k, b) => k < bound by idtac=>/#. case (b1) => hb1. elim H22. progress. elim H22. progress. rewrite (H24 k b1). done. progress. smt. progress. smt. elim H22. progress. elim H22. progress. rewrite (H24 k b1). done. progress. smt. progress. smt. *)
 
-
-    rcondt{1} 12. auto. while (0 <= i <= DKCp.l). if. auto => /#. auto => /#. wp. while true. auto. auto. progress => /#. rcondt{1} 12. progress. while (0 <= i <= DKCp.l). if. auto => /#. auto => /#. wp. while true. auto. auto. progress => /#. rcondf{1} 17. progress. auto. while (0 <= i <= DKCp.l). if. auto => /#. auto => /#. wp. while true. auto. auto. progress => /#. 
+    rcondt{1} 13. auto. while (0 <= i <= DKCp.l). if. auto => /#. auto => /#. wp. while true. auto. auto. progress;smt. rcondt{1} 13. progress. while (0 <= i <= DKCp.l). if. auto => /#. auto => /#. wp. while true. auto. auto. progress;smt. rcondf{1} 18. progress. auto. while (0 <= i <= DKCp.l). if. auto => /#. auto => /#. wp. while true. auto. auto. progress;smt.
     
-    rcondt{2} 13. auto. while (0 <= i <= Param.l). if. auto => /#. auto => /#. wp. while true. auto. auto. progress => /#. rcondt{2} 13. progress. while (0 <= i <= Param.l). if. auto => /#. auto => /#. wp. while true. auto. auto. progress => /#. rcondf{2} 18. progress. auto. while (0 <= i <= Param.l). if. auto => /#. auto => /#. wp. while true. auto. auto. progress => /#. 
+    rcondt{2} 13. auto. while (0 <= i <= Param.l). if. auto => /#. auto => /#. wp. while true. auto. auto. progress;smt. rcondt{2} 13. progress. while (0 <= i <= Param.l). if. auto => /#. auto => /#. wp. while true. auto. auto. progress;smt. rcondf{2} 18. progress. auto. while (0 <= i <= Param.l). if. auto => /#. auto => /#. wp. while true. auto. auto. progress;smt. 
 
     swap{2} 1 12.
     wp. rnd (fun w, fst (w2kw' w)) (fun w, kw2w' w (!Param.lsb{2})). wp. rnd (fun w, fst (w2kw' w)) (fun w, kw2w' w (Param.lsb{2})). rnd.
@@ -430,7 +422,13 @@ equiv true_key lp (A <:  Adv_DKC_t{Param,DKCp,PRFr_Wrapped}):
       (*snd (oget Param.kpub{2}.[(Param.l{2},Param.lsb{2})]) = Param.lsb{2} /\*)
       (forall k b, 0 <= k < i{1} => k <> Param.l{2} => oget DKCp.kpub{1}.[(k,b)] = kw2w (fst (oget Param.kpub{2}.[(k,b)])) b) /\
       (forall k b, 0 <= k < i{1} => snd (oget Param.kpub{2}.[(k,b)]) = b) /\
-      (forall k, 0 <= k < i{1} => k = Param.l{2} => oget DKCp.kpub{1}.[(k,!Param.lsb{2})] = kw2w (fst (oget Param.kpub{2}.[(k,!Param.lsb{2})])) (!Param.lsb{2}))).
+      (forall k, 0 <= k < i{1} => k = Param.l{2} => oget DKCp.kpub{1}.[(k,!Param.lsb{2})] = kw2w (fst (oget Param.kpub{2}.[(k,!Param.lsb{2})])) (!Param.lsb{2})) 
+      (*(forall k b, 0 <= k < i{1} => k <> Param.l{2} => mem (dom DKCp.kpub{1}) (k,b)) /\
+      (forall k b, 0 <= k < i{1} => k <> Param.l{2} => mem (dom Param.kpub{2}) (k,b)) /\
+      (forall k, 0 <= k < i{1} => k = Param.l{2} => mem (dom DKCp.kpub{1}) (k, !Param.lsb{2})) /\
+      (forall k, 0 <= k < i{1} => k = Param.l{2} => mem (dom Param.kpub{2}) (k, !Param.lsb{2})) /\
+      (forall k b, mem (dom DKCp.kpub{1}) (k,b) => 0 <= k < bound) /\
+      (forall k b, mem (dom Param.kpub{2}) (k,b) => 0 <= k < bound)*)).
 
     rcondf{1} 1. auto. progress => /#.
     rcondf{2} 1. auto. progress => /#.
@@ -440,6 +438,17 @@ equiv true_key lp (A <:  Adv_DKC_t{Param,DKCp,PRFr_Wrapped}):
         rewrite !getP. case ((k, b1) = (i{2}, true)) => hc. rewrite oget_some. simplify w2kw snd. rewrite (Dword.lsb_dwordLsb (true) _). done. idtac=>/#. case ((k, b1) = (i{2}, false)) => hc'. rewrite oget_some. simplify w2kw snd. rewrite (Dword.lsb_dwordLsb (false) _). done. idtac=>/#. idtac=>/#. 
         rewrite !getP => /#.  
 
+        (*rewrite !dom_set. rewrite !in_fsetU. case (k = i{2}) => hki. case (b1) => hb1. right. rewrite in_fset1. done. left. right. rewrite in_fset1. done. left. left. rewrite H8. idtac=>/#. done. 
+        rewrite !dom_set. rewrite !in_fsetU. case (k = i{2}) => hki. case (b1) => hb1. right. rewrite in_fset1. done. left. right. rewrite in_fset1. done. left. left. rewrite H9. idtac=>/#. done. 
+        rewrite !dom_set. rewrite !in_fsetU. left. left. rewrite H10. idtac=>/#. done.  
+        rewrite !dom_set. rewrite !in_fsetU. left. left. rewrite H11. idtac=>/#. done.
+    
+        move : H22. rewrite !dom_set. rewrite !in_fsetU. progress. cut ? : forall (k : int) (b : bool), mem (dom DKCp.kpub{1}) (k, b) => 0 <= k by idtac=>/#. case (b1) => hb1. elim H22. progress. elim H22. progress. rewrite (H23 k b1). done. progress. smt. progress. smt. elim H22. progress. elim H22. progress. rewrite (H23 k b1). done. progress. smt. progress. smt. 
+        move : H22. rewrite !dom_set. rewrite !in_fsetU. progress. cut ? : forall (k : int) (b : bool), mem (dom DKCp.kpub{1}) (k, b) => k < bound by idtac=>/#. case (b1) => hb1. elim H22. progress. elim H22. progress. rewrite (H24 k b1). done. progress. smt. progress. smt. elim H22. progress. elim H22. progress. rewrite (H24 k b1). done. progress. smt. progress. smt. 
+        move : H22. rewrite !dom_set. rewrite !in_fsetU. progress. cut ? : forall (k : int) (b : bool), mem (dom Param.kpub{2}) (k, b) => 0 <= k by idtac=>/#. case (b1) => hb1. elim H22. progress. elim H22. progress. rewrite (H23 k b1). done. progress. smt. progress. smt. elim H22. progress. elim H22. progress. rewrite (H23 k b1). done. progress. smt. progress. smt. 
+        move : H22. rewrite !dom_set. rewrite !in_fsetU. progress. cut ? : forall (k : int) (b : bool), mem (dom Param.kpub{2}) (k, b) => k < bound by idtac=>/#. case (b1) => hb1. elim H22. progress. elim H22. progress. rewrite (H24 k b1). done. progress. smt. progress. smt. elim H22. progress. elim H22. progress. rewrite (H24 k b1). done. progress. smt. progress. smt. *)
+
+    
     wp; while (={glob A} /\ 0 <= lp < bound /\ b{1} /\ ={i} /\ 0 <= i{1} <= bound /\ (b{1}, l{1}).`2 = lp /\ l{2} = lp /\
       DKCp.used{1} = Param.used{2} /\ DKCp.used{1} = fset0 /\ DKCp.b{1} = b{1} /\ DKCp.b{1} /\
       DKCp.l{1} = Param.l{2} /\ DKCp.l{1} = lp /\ Param.l{2} = l0{2} /\ DKCp.l{1} = l{1} /\
@@ -448,11 +457,23 @@ equiv true_key lp (A <:  Adv_DKC_t{Param,DKCp,PRFr_Wrapped}):
       (forall k, 0 <= k < i{1} => oget DKCp.kpub{1}.[(k,false)] = W.zeros) /\
       (forall k, 0 <= k < i{1} => oget DKCp.kpub{1}.[(k,true)] = W.zeros) /\
       (forall k, 0 <= k < i{1} => oget Param.kpub{2}.[(k,false)] = (KW.zeros, false)) /\
-      (forall k, 0 <= k < i{1} => oget Param.kpub{2}.[(k,true)] = (KW.zeros, true))).
+      (forall k, 0 <= k < i{1} => oget Param.kpub{2}.[(k,true)] = (KW.zeros, true))
+      (*(forall k b, 0 <= k < i{1} => mem (dom DKCp.kpub{1}) (k,b)) /\
+      (forall k b, 0 <= k < i{1} => mem (dom Param.kpub{2}) (k,b)) /\
+      (forall k b, mem (dom DKCp.kpub{1}) (k,b) => 0 <= k < i{1}) /\
+      (forall k b, mem (dom Param.kpub{2}) (k,b) => 0 <= k < i{1})*)).
       auto; progress; expect 6 by by rewrite ?getP => /#. 
+(*        rewrite !dom_set. rewrite !in_fsetU. case (k = i{2}) => hki. case (b1) => hb1. right. rewrite in_fset1. done. left. right. rewrite in_fset1. done. left. left. rewrite H9. idtac=>/#. 
+        rewrite !dom_set. rewrite !in_fsetU. case (k = i{2}) => hki. case (b1) => hb1. right. rewrite in_fset1. done. left. right. rewrite in_fset1. done. left. left. rewrite H10. idtac=>/#. 
+    
+       move : H15. rewrite !dom_set. rewrite !in_fsetU. progress. cut ? : forall (k : int) (b : bool), mem (dom DKCp.kpub{1}) (k, b) => 0 <= k by idtac=>/#. case (b1) => hb1. elim H15. progress. elim H15. progress. rewrite (H16 k b1). done. progress. smt. progress. smt. elim H15. progress. elim H15. progress. rewrite (H16 k b1). done. progress. smt. progress. smt. 
+        move : H15. rewrite !dom_set. rewrite !in_fsetU. progress. cut ? : forall (k : int) (b : bool), mem (dom DKCp.kpub{1}) (k, b) => k < i{2} + 1 by idtac=>/#. case (b1) => hb1. elim H15. progress. elim H15. progress. rewrite (H17 k b1). done. progress. smt. progress. smt. elim H15. progress. elim H15. progress. rewrite (H17 k b1). done. progress. smt. progress. smt. 
+        move : H15. rewrite !dom_set. rewrite !in_fsetU. progress. cut ? : forall (k : int) (b : bool), mem (dom Param.kpub{2}) (k, b) => 0 <= k by idtac=>/#. case (b1) => hb1. elim H15. progress. elim H15. progress. rewrite (H16 k b1). done. progress. smt. progress. smt. elim H15. progress. elim H15. progress. rewrite (H16 k b1). done. progress. smt. progress. smt. 
+        move : H15. rewrite !dom_set. rewrite !in_fsetU. progress. cut ? : forall (k : int) (b : bool), mem (dom Param.kpub{2}) (k, b) => k < i{2} + 1 by idtac=>/#. case (b1) => hb1. elim H15. progress. elim H15. progress. rewrite (H17 k b1). done. progress. smt. progress. smt. elim H15. progress. elim H15. progress. rewrite (H17 k b1). done. progress. smt. progress. smt. *)
 
     auto; progress; last 3 by idtac=>/#.
         by smt. 
+        by smt.
         by rewrite map0P =>/#.
         by rewrite map0P =>/#.
         by rewrite map0P =>/#.
@@ -470,12 +491,27 @@ equiv true_key lp (A <:  Adv_DKC_t{Param,DKCp,PRFr_Wrapped}):
         rewrite kw2w'_w2kw'. by rewrite (Dword.lsb_dwordLsb (!lsbL) _). done.  
         rewrite kw2w_w2kw'. by rewrite (Dword.lsb_dwordLsb (lsbL) _). done.  
         by rewrite (Dword.lsb_dwordLsb (lsbL) _). 
-        by smt.
+        by idtac=>/#.
         by idtac=>/#.
         by rewrite !getP => /#. 
         by rewrite !getP => /#. 
         by rewrite !getP => /#. 
         rewrite !getP. case ((l{1}, !lsbL) = (i_R0, !lsbL)) => hc. rewrite !oget_some. smt. case ((l{1}, !lsbL) = (i_R0, lsbL)) => hc'. smt. idtac=>/#. 
+        (*rewrite !dom_set. rewrite !in_fsetU. case (k = i_R0) => hki. case (b1 = !lsbL) => hb1. right. rewrite in_fset1. done. left. right. rewrite in_fset1. idtac=>/#. left. left. rewrite H29. idtac=>/#. done.
+        rewrite !dom_set. rewrite !in_fsetU. case (k = i_R0) => hki. case (b1 = !lsbL) => hb1. right. rewrite in_fset1. done. left. right. rewrite in_fset1. idtac=>/#. left. left. rewrite H30. idtac=>/#. done.
+        by smt. 
+        by smt.
+
+        move : H47. rewrite !dom_set. rewrite !in_fsetU. progress. cut ? : forall (k : int) (b : bool), mem (dom kpub_L0) (k, b) => 0 <= k by idtac=>/#. case (b1) => hb1. elim H47. progress. elim H47. progress. rewrite (H48 k b1). done. progress. smt. progress. smt. elim H47. progress. elim H47. progress. rewrite (H48 k b1). done. progress. smt. progress. smt. 
+        move : H47. rewrite !dom_set. rewrite !in_fsetU. progress. cut ? : forall (k : int) (b : bool), mem (dom kpub_L0) (k, b) => k < bound by idtac=>/#. case (b1) => hb1. elim H47. progress. elim H47. progress. rewrite (H49 k b1). done. progress. smt. progress. smt. elim H47. progress. elim H47. progress. rewrite (H49 k b1). done. progress. smt. progress. smt. 
+        move : H47. rewrite !dom_set. rewrite !in_fsetU. progress. cut ? : forall (k : int) (b : bool), mem (dom kpub_R0) (k, b) => 0 <= k by idtac=>/#. case (b1) => hb1. elim H47. progress. elim H47. progress. rewrite (H48 k b1). done. progress. smt. progress. smt. elim H47. progress. elim H47. progress. rewrite (H48 k b1). done. progress. smt. progress. smt. 
+        move : H47. rewrite !dom_set. rewrite !in_fsetU. progress. cut ? : forall (k : int) (b : bool), mem (dom kpub_R0) (k, b) => k < bound by idtac=>/#. case (b1) => hb1. elim H47. progress. elim H47. progress. rewrite (H49 k b1). done. progress. smt. progress. smt. elim H47. progress. elim H47. progress. rewrite (H49 k b1). done. progress. smt. progress. smt. 
+    
+by idtac=>/#.
+by idtac=>/#.
+by idtac=>/#.
+by idtac=>/#.*)
+
         wp. 
 
     call (_: 
@@ -503,24 +539,38 @@ equiv true_key lp (A <:  Adv_DKC_t{Param,DKCp,PRFr_Wrapped}):
     0 <= k < bound =>
     k = Param.l{2} =>
     oget DKCp.kpub{1}.[(k, !Param.lsb{2})] =
-    kw2w (fst (oget Param.kpub{2}.[(k, !Param.lsb{2})])) (!Param.lsb{2}))).
+    kw2w (fst (oget Param.kpub{2}.[(k, !Param.lsb{2})])) (!Param.lsb{2}))
+  (*(forall (k : int) (b0 : bool),
+     0 <= k < bound => k <> Param.l{2} => mem (dom DKCp.kpub{1}) (k, b0)) /\
+  (forall (k : int) (b0 : bool),
+     0 <= k < bound => k <> Param.l{2} => mem (dom Param.kpub{2}) (k, b0)) /\
+  (forall (k : int),
+     0 <= k < bound =>
+     k = Param.l{2} => mem (dom DKCp.kpub{1}) (k, !Param.lsb{2})) /\
+  (forall (k : int),
+     0 <= k < bound =>
+     k = Param.l{2} => mem (dom Param.kpub{2}) (k, !Param.lsb{2})) /\
+  (forall (k : int) (b0 : bool),
+     mem (dom DKCp.kpub{1}) (k, b0) => 0 <= k < bound) /\
+  (forall (k : int) (b0 : bool),
+    mem (dom Param.kpub{2}) (k, b0) => 0 <= k < bound)*)).
 
     proc.
-    case (! mem DKCp.used{1} q{1}.`5 && 0 <= q{1}.`2.`1 /\       
-    q{1}.`2.`1 < q{1}.`3.`1 &&                 
-    q{1}.`3.`1 < q{1}.`4.`1 &&      q{1}.`4.`1 < bound /\             
+    case (! mem DKCp.used{1} q{1}.`5 /\ 0 <= q{1}.`2.`1 /\
+    q{1}.`2.`1 < q{1}.`3.`1 /\       
+    q{1}.`3.`1 < q{1}.`4.`1 /\  q{1}.`4.`1 < bound /\                
     q{1}.`4 <> (DKCp.l{1}, DKCp.lsb{1})); last first.
 
-      rcondf{1} 3; first by auto. 
-      rcondf{2} 3; first by auto. 
+      rcondf{1} 3; first by auto.
+      rcondf{2} 3; first by auto.   
       by auto.
 
       rcondt{1} 3; first by auto. 
       rcondt{2} 3; first by auto.
  
       case (q{1}.`1).
-        rcondt{1} 8. auto => /#. 
-        rcondt{2} 8. auto. 
+        rcondt{1} 8; first by auto => /#. 
+        rcondt{2} 8; first by auto. 
 
     case (q{2}.`2 = (Param.l{2}, Param.lsb{2})).
         rcondt{2} 9. progress. auto. 
@@ -528,7 +578,7 @@ equiv true_key lp (A <:  Adv_DKC_t{Param,DKCp,PRFr_Wrapped}):
         wp. rnd. wp. skip. progress. 
         by rewrite H14 H3 => /#.   
 
-          cut ->: q{2}.`3 = (q{2}.`3.`1,q{2}.`3.`2) by idtac=>/#. rewrite H4 => /#.
+          cut ->: q{2}.`3 = (q{2}.`3.`1,q{2}.`3.`2) by idtac=>/#. rewrite H4 => /#. 
           simplify PrfDKC.E. simplify PRF.F. rewrite H14 /=. congr. congr. congr. rewrite w2kw_kw2w => /#. cut ->: q{2}.`3 = (q{2}.`3.`1,q{2}.`3.`2) by idtac=>/#. rewrite H4. idtac=>/#. idtac=>/#. rewrite w2kw_kw2w =>/#. 
 
     case (q{2}.`3 = (Param.l{2}, Param.lsb{2})).
@@ -563,7 +613,7 @@ equiv true_key lp (A <:  Adv_DKC_t{Param,DKCp,PRFr_Wrapped}):
         by rewrite H14 H3 => /#.   
 
           cut ->: q{2}.`3 = (q{2}.`3.`1,q{2}.`3.`2) by idtac=>/#. rewrite H4 => /#.
-          simplify PrfDKC.E. simplify PRF.F. rewrite H14 /=. congr. congr. congr. rewrite w2kw_kw2w => /#. cut ->: q{2}.`3 = (q{2}.`3.`1,q{2}.`3.`2) by idtac=>/#. rewrite H4. idtac=>/#. idtac=>/#. rewrite w2kw_kw2w =>/#. idtac=>/#.
+          simplify PrfDKC.E. simplify PRF.F. rewrite H14 /=. congr. congr. congr. rewrite w2kw_kw2w => /#. cut ->: q{2}.`3 = (q{2}.`3.`1,q{2}.`3.`2) by idtac=>/#. rewrite H4. idtac=>/#. idtac=>/#. rewrite w2kw_kw2w =>/#. cut ->: q{2}.`4 = (q{2}.`4.`1,q{2}.`4.`2) by idtac=>/#. rewrite H4. idtac=>/#. idtac=>/#. idtac=>/#.
 
     case (q{2}.`3 = (Param.l{2}, Param.lsb{2})).
         rcondf{2} 8. progress. auto. rcondt{2} 8. progress. auto. 
@@ -590,7 +640,7 @@ equiv true_key lp (A <:  Adv_DKC_t{Param,DKCp,PRFr_Wrapped}):
       
 equiv false_key lp (A <:  Adv_DKC_t{Param,DKCp,PRFr_Wrapped,RandomFunction}):
     DKCSecurity.Game(DKC_O,A).game ~
-    IND(RandomFunction,D(A)).main : ={glob A} /\ 0 <= lp < bound /\ !b{1} /\ l{1} = lp /\ l{2} = lp
+    IND(RandomFunction,D(A)).main : ={glob A} /\ 0 <= lp < boundl /\ !b{1} /\ l{1} = lp /\ l{2} = lp
                                ==> res{1} <> res{2}.
 
     proof.
@@ -615,8 +665,8 @@ equiv false_key lp (A <:  Adv_DKC_t{Param,DKCp,PRFr_Wrapped,RandomFunction}):
     );   
       inline DKC_O.initialize D(A, RandomFunction).initialize.
 
-        splitwhile{1} 11 : i < DKCp.l. 
-        splitwhile{1} 12 : i = DKCp.l.
+        splitwhile{1} 12 : i < DKCp.l. 
+        splitwhile{1} 13 : i = DKCp.l.
     
         splitwhile{2} 12 : i < Param.l. 
         splitwhile{2} 13 : i = Param.l.
@@ -644,9 +694,9 @@ equiv false_key lp (A <:  Adv_DKC_t{Param,DKCp,PRFr_Wrapped,RandomFunction}):
         rewrite !getP => /#. 
 
 
-    rcondt{1} 12. auto. while (0 <= i <= DKCp.l). if. auto => /#. auto => /#. wp. while true. auto. auto. progress => /#. rcondt{1} 12. progress. while (0 <= i <= DKCp.l). if. auto => /#. auto => /#. wp. while true. auto. auto. progress => /#. rcondf{1} 17. progress. auto. while (0 <= i <= DKCp.l). if. auto => /#. auto => /#. wp. while true. auto. auto. progress => /#. 
+    rcondt{1} 13. auto. while (0 <= i <= DKCp.l). if. auto => /#. auto => /#. wp. while true. auto. auto. progress;smt. rcondt{1} 13. progress. while (0 <= i <= DKCp.l). if. auto => /#. auto => /#. wp. while true. auto. auto. progress;smt. rcondf{1} 18. progress. auto. while (0 <= i <= DKCp.l). if. auto => /#. auto => /#. wp. while true. auto. auto. progress;smt. 
     
-    rcondt{2} 13. auto. while (0 <= i <= Param.l). if. auto => /#. auto => /#. wp. while true. auto. auto. progress => /#. rcondt{2} 13. progress. while (0 <= i <= Param.l). if. auto => /#. auto => /#. wp. while true. auto. auto. progress => /#. rcondf{2} 18. progress. auto. while (0 <= i <= Param.l). if. auto => /#. auto => /#. wp. while true. auto. auto. progress => /#. 
+    rcondt{2} 13. auto. while (0 <= i <= Param.l). if. auto => /#. auto => /#. wp. while true. auto. auto. progress;smt. rcondt{2} 13. progress. while (0 <= i <= Param.l). if. auto => /#. auto => /#. wp. while true. auto. auto. progress;smt. rcondf{2} 18. progress. auto. while (0 <= i <= Param.l). if. auto => /#. auto => /#. wp. while true. auto. auto. progress;smt. 
 
     wp. rnd (fun w, fst (w2kw' w)) (fun w, kw2w' w (!Param.lsb{2})). wp. rnd{1}. rnd.
     
@@ -683,7 +733,8 @@ equiv false_key lp (A <:  Adv_DKC_t{Param,DKCp,PRFr_Wrapped,RandomFunction}):
       auto; progress; expect 6 by by rewrite ?getP => /#. 
 
     auto; progress; last 3 by idtac=>/#.
-        by smt. 
+        by smt.
+        by smt.
         by rewrite map0P =>/#.
         by rewrite map0P =>/#.
         by rewrite map0P =>/#.
@@ -732,12 +783,12 @@ equiv false_key lp (A <:  Adv_DKC_t{Param,DKCp,PRFr_Wrapped,RandomFunction}):
     proc.
     
     case (! mem DKCp.used{1} q{1}.`5 && 0 <= q{1}.`2.`1 /\       
-    q{1}.`2.`1 < q{1}.`3.`1 &&                 
-    q{1}.`3.`1 < q{1}.`4.`1 &&      q{1}.`4.`1 < bound /\             
+    q{1}.`2.`1 < q{1}.`3.`1 /\                 
+    q{1}.`3.`1 < q{1}.`4.`1 /\      q{1}.`4.`1 < bound /\             
     q{1}.`4 <> (DKCp.l{1}, DKCp.lsb{1})); last first.
 
-      rcondf{1} 3; first by auto. 
-      rcondf{2} 3; first by auto. 
+      rcondf{1} 3; first by auto => /#. 
+      rcondf{2} 3; first by auto => /#. 
       by auto.
 
       rcondt{1} 3; first by auto. 
@@ -782,7 +833,7 @@ equiv false_key lp (A <:  Adv_DKC_t{Param,DKCp,PRFr_Wrapped,RandomFunction}):
       rcondt{2} 10. auto.  
     wp. rnd{2}. wp. rnd. wp. skip. progress. 
       by smt.
-      cut ->: q{2}.`2 = (q{2}.`2.`1,q{2}.`2.`2) by idtac=>/#. idtac=>/#.
+      cut ->: q{2}.`2 = (q{2}.`2.`1,q{2}.`2.`2) by idtac=>/#. smt tmo=10.
       cut ->: q{2}.`3 = (q{2}.`3.`1,q{2}.`3.`2) by idtac=>/#. smt tmo=10. 
       cut ->: q{2}.`2 = (Param.l{2}, getlsb DKCp.ksec{1}) <=> false by idtac=>/#. cut ->: q{2}.`3 = (Param.l{2}, getlsb DKCp.ksec{1}) <=> false by idtac=>/#. simplify. simplify E. congr. congr. congr. cut ->: q{2}.`2 = (q{2}.`2.`1,q{2}.`2.`2) by idtac=>/#. by smt. by smt. 
       by rewrite dom_set.  
@@ -825,15 +876,14 @@ equiv false_key lp (A <:  Adv_DKC_t{Param,DKCp,PRFr_Wrapped,RandomFunction}):
     wp. rnd{2}. wp. skip. progress. 
       by smt.
       cut ->: q{2}.`2 = (q{2}.`2.`1,q{2}.`2.`2) by idtac=>/#. idtac=>/#. 
-      cut ->: q{2}.`3 = (q{2}.`3.`1,q{2}.`3.`2) by idtac=>/#. idtac=>/#. 
+      cut ->: q{2}.`3 = (q{2}.`3.`1,q{2}.`3.`2) by idtac=>/#. smt tmo=10.  
       cut ->: q{2}.`2 = (Param.l{2}, getlsb DKCp.ksec{1}) <=> false by idtac=>/#. cut ->: q{2}.`3 = (Param.l{2}, getlsb DKCp.ksec{1}) <=> false by idtac=>/#. simplify. simplify E. congr. congr. congr. cut ->: q{2}.`2 = (q{2}.`2.`1,q{2}.`2.`2) by idtac=>/#. by smt. by smt. simplify. cut ->: q{2}.`4 = (q{2}.`4.`1,q{2}.`4.`2) by idtac=>/#. case (q{2}.`4.`1 = Param.l{2}) => hc. cut ->: q{2}.`4.`2 = ! getlsb DKCp.ksec{1} by idtac=>/#. rewrite H5 => /#. rewrite H3 => /#.
       by rewrite dom_set.  
     
 skip. progress. by rewrite dom0. idtac=>/#. 
   qed.
-
     
-lemma PrfDKC_secure (A <: Adv_DKC_t{PRFr_Wrapped,DKCp,Param,RandomFunction}) &m i: 0 <= i < bound =>
+lemma PrfDKC_secure (A <: Adv_DKC_t{PRFr_Wrapped,DKCp,Param,RandomFunction}) &m i: 0 <= i < boundl =>
     Pr[DKCSecurity.Game(DKC_O,A).game(true,i)@ &m:res] - 
     Pr[DKCSecurity.Game(DKC_O,A).game(false,i)@ &m:!res] =
     Pr[IND(PRFr_Wrapped,D(A)).main(i)@ &m:res] - Pr[IND(RandomFunction,D(A)).main(i)@ &m:res].
@@ -843,6 +893,5 @@ lemma PrfDKC_secure (A <: Adv_DKC_t{PRFr_Wrapped,DKCp,Param,RandomFunction}) &m 
     byequiv (true_key (i) A). done. done.
     congr. byequiv (false_key (i) A). done. smt. 
 qed.
-
   
 end SomeDKC.
